Arithmetic/theories/Semantics.v
@@ -8,8 +8,8 @@ Open Scope Z_scope.
 
 Definition exp_sem_sig {T : Set} : Type := Env -> @_c_exp T -> 𝕍 -> Prop.
 Definition stmt_sem_sig {S T: Set} : Type  :=  @fenv S T -> Env -> @_c_statement S T ->  Env -> Prop.
-Definition Empty_exp_sem : @exp_sem_sig Empty_set := fun _ _ _ => False.
-Definition Empty_stmt_sem : @stmt_sem_sig Empty_set Empty_set := fun _ _ _ _ => False.
+Definition Empty_exp_sem {T: Set} : @exp_sem_sig T := fun _ _ _ => False.
+Definition Empty_stmt_sem {S T: Set} : @stmt_sem_sig S T := fun _ _ _ _ => False.
 
 Declare Scope generic_exp_sem_scope.
 Delimit Scope generic_exp_sem_scope with gesem.
@@ -35,7 +35,7 @@ Inductive generic_exp_sem {T:Set} {ext_exp : @exp_sem_sig T} (ev:Env): @_c_exp T
     ev |= e' => VInt (z' ⁱⁿᵗ z'_ir) -> 
     ((◁ op) z z' = false ) ->
     ev |= BinOpBool e op e' => VInt zero
-| C_Ext x v t: 
+(* | C_Ext x v t: 
     (* variable must not be of type int (treated by C_E_Var) *)
     t <> C_Int ->
     
@@ -46,7 +46,7 @@ Inductive generic_exp_sem {T:Set} {ext_exp : @exp_sem_sig T} (ev:Env): @_c_exp T
     (* the external semantic can only add additional constraint, the result is always v *)
     ext_exp ev (C_Id x t) v ->
 
-    ev |= (C_Id x t) => v
+    ev |= (C_Id x t) => v *)
 
 where  "env '|=' e => z" := (generic_exp_sem env e z) : generic_exp_sem_scope.
 
@@ -59,21 +59,7 @@ Delimit Scope c_sem_scope with csem.
 
 Definition c_exp_sem := @generic_exp_sem Empty_set Empty_exp_sem.
 
-Notation "Ω |= e => v"  := (c_exp_sem Ω ⊥ e v) : c_sem_scope.
-
-Inductive _gmp_exp_sem (ev:Env) : gmp_exp -> 𝕍 -> Prop :=
-| GMP_E_Var (x:𝓥) (l:location) (z:mpz_val) : 
-    ev x = Some (Def l) -> 
-    ev.(mstate) l = Some z ->
-    _gmp_exp_sem ev (C_Id x Mpz) (VMpz l)
-.
-
-#[global] Hint Constructors _gmp_exp_sem  : rac_hint.
-
-Declare Scope gmp_exp_sem_scope.
-Delimit Scope gmp_exp_sem_scope with gmpesem.
-Definition gmp_exp_sem := @generic_exp_sem _gmp_t _gmp_exp_sem.
-Notation "ev '|=' e => z" := (gmp_exp_sem ev e z) : gmp_exp_sem_scope.
+Notation "Ω '|=' e => v"  := (c_exp_sem Ω e v) : c_sem_scope.
 
 Open Scope mini_c_scope.
 From RecordUpdate Require Import RecordUpdate.
@@ -165,7 +151,6 @@ Notation "ev |= s => ev'"  := (c_stmt_sem ev s ev') : c_sem_scope. *)
          *)
 
 
-Open Scope gmp_exp_sem_scope.
 Open Scope mini_gmp_scope.
 Declare Scope gmp_stmt_sem_scope.
 Delimit Scope gmp_stmt_sem_scope with gmpssem.
@@ -184,7 +169,7 @@ Inductive _gmp_stmt_sem { S T : Set } (f : @fenv S T) (ev:Env) : gmp_statement -
 
     | S_set_i x y z a :  
         ev x = Some (Def (VMpz (Some a))) ->
-        (ev |= y => VInt z)%gmpesem ->
+        (ev |= y => VInt z)%csem ->
         (ev |= <(set_i(x,y))> => ev <| mstate ::= {{a\Defined (z ̇)}} |>) f
 
     | S_set_z x y z (a n : location) :  
@@ -193,35 +178,35 @@ Inductive _gmp_stmt_sem { S T : Set } (f : @fenv S T) (ev:Env) : gmp_statement -
         ev.(mstate) n = Some z ->
         (ev |= <(set_z(x,y))> => ev <| mstate ::= {{a\z}} |>) f 
 
-    | S_get_int x (y:id) z v (ir:Int.inRange z) :
-        (ev |= C_Id y Mpz => VMpz (Some v))%gmpesem ->
-        ev.(mstate) v = Some (Defined z) -> 
-        (ev |= <(x = get_int(y))> => ev <| env ; vars ::= {{x\VInt (z ⁱⁿᵗ ir) : 𝕍}} |>) f
+    | S_get_int x y ly zy (ir:Int.inRange zy) :
+        ev y = Some (Def (VMpz (Some ly))) ->
+        ev.(mstate) ly = Some (Defined zy) -> 
+        (ev |= <(x = get_int(y))> => ev <| env ; vars ::= {{x\VInt (zy ⁱⁿᵗ ir) : 𝕍}} |>) f
 
-    | S_set_s s x z a :
-        ev x = Some (Def (VMpz (Some a))) ->
-        BinaryString.to_Z s = z ->
-        (ev |= <(set_s(x,s))> => ev <| mstate ::= {{a\Defined z}} |> ) f
+    | S_set_s s x zx lx :
+        ev x = Some (Def (VMpz (Some lx))) ->
+        BinaryString.to_Z s = zx ->
+        (ev |= <(set_s(x,s))> => ev <| mstate ::= {{lx\Defined zx}} |> ) f
 
-    | S_cmp c x (vx vy :location) lx y ly (b:𝕍):
-        (ev |= C_Id x Mpz => vx)%gmpesem ->
-        (ev |= C_Id y Mpz => vy)%gmpesem ->
-        ev.(mstate) vx = Some (Defined lx) ->
-        ev.(mstate) vy = Some (Defined ly) ->
+    | S_cmp c x (lx ly :location) zx y zy (b:𝕍):
+        ev x = Some (Def (VMpz (Some lx))) ->
+        ev y = Some (Def (VMpz (Some ly))) ->
+        ev.(mstate) lx = Some (Defined zx) ->
+        ev.(mstate) ly = Some (Defined zy) ->
         (
-            (Z.gt lx ly <-> b = VInt one) /\
-            (Z.lt lx ly <-> b = VInt sub_one) /\
-            (Z.eq lx ly <-> b = VInt zero)
+            (Z.gt zx zy <-> b = VInt one) /\
+            (Z.lt zx zy <-> b = VInt sub_one) /\
+            (Z.eq zx zy <-> b = VInt zero)
         ) ->
         (ev |= <(c = cmp(x,y))> => ev <| env ; vars ::= {{c\b}} |>) f
     
-    | S_op bop r lr x y (vx vy : location) z1 z2 :
-        (ev |= C_Id x Mpz => vx)%gmpesem ->
-        ev.(mstate) vx = Some (Defined z1) -> 
-        (ev |= C_Id y Mpz =>  vy)%gmpesem ->
-        ev.(mstate) vy = Some (Defined z2) -> 
-        ev r = Some (Def (VMpz (Some lr))) ->
-        (ev |= op bop r x y => ev <| mstate ::= {{lr\Defined (⋄ (□ bop) z1 z2) }} |>) f
+    | S_op bop r lr x y (lx ly : location) zx zy :
+        ev x = Some (Def (VMpz (Some lx))) ->
+        ev y = Some (Def (VMpz (Some ly))) ->
+        ev.(mstate) lx = Some (Defined zx) ->
+        ev.(mstate) ly = Some (Defined zy) ->
+        ev r = Some (Def (VMpz (Some lr))) -> (* not in paper *)
+        (ev |= op bop r x y => ev <| mstate ::= {{lr\Defined (⋄ (□ bop) zx zy) }} |>) f
 
 where "ev |= s => ev'" := (fun f => _gmp_stmt_sem f ev s ev') : gmp_stmt_sem_scope.
 
@@ -230,7 +215,7 @@ where "ev |= s => ev'" := (fun f => _gmp_stmt_sem f ev s ev') : gmp_stmt_sem_sco
 
 
 
-Definition gmp_stmt_sem := @generic_stmt_sem _gmp_statement _gmp_t _gmp_exp_sem _gmp_stmt_sem.
+Definition gmp_stmt_sem := @generic_stmt_sem _gmp_statement _gmp_t Empty_exp_sem _gmp_stmt_sem.
 (*
 Notation "Ω ⋅ M |= s => Ω' ⋅ M'"  := (fun f => gmp_stmt_sem f Ω M s Ω' M') : gmp_sem_scope. 
  *)
@@ -329,18 +314,41 @@ Notation "ev |= s => ev'"  := (fun f => fsl_stmt_sem f ev s ev') : fsl_sem_scope
 
 
 
-(* macro semantic *)
+(* macro semantic, section E *)
 
 
 Declare Scope macro_sem_scope.
 Inductive macro_sem (ev:Env) (e:gmp_exp): Z -> Prop :=
-| M_Int x :  
-    gmp_exp_sem ev e (VInt x) ->
+| M_Int x : 
+    ty e = C_Int -> 
+    (ev |= gmp_exp_to_c_exp e => (VInt x))%csem ->
     ev |= e ⇝ x ̇
 | M_Mpz l z : 
-    gmp_exp_sem ev e (VMpz (Some l)) ->
+    ty e = Mpz ->
+    ev (gmp_ty_mpz_to_var e) = Some (Def (VMpz (Some l))) ->
     ev.(mstate) l = Some (Defined z) ->
     ev |= e ⇝ z
 where "ev '|=' e ⇝ z" := (macro_sem ev e z) : macro_sem_scope.
 
 #[global] Hint Constructors macro_sem : rac_hint.
+
+
+
+(* misc *)
+Require Import Coq.Program.Equality. (* axiom eq_rect_eq *)
+
+Fact ty_int_gmp_c_exp_equiv {ext_exp} (e:gmp_exp): forall env v, 
+    ty e = C_Int -> 
+    (env |= gmp_exp_to_c_exp e => v)%csem <-> generic_exp_sem env e v (ext_exp:=ext_exp).
+Proof with eauto with rac_hint.
+    intros env v Hint. split; intro H.
+    - dependent induction H; destruct e eqn:E; simpl in *; subst; try congruence; injection x as Hz; subst.
+        1,2: now constructor.
+        1,2,3: destruct (ty g1) eqn:TG1; try discriminate ; destruct (ty g2) eqn:TG2; try discriminate...
+    - induction H ; simpl in *.
+        1,2: now repeat constructor.
+        1,2,3: destruct (ty e) eqn:TE1; try discriminate ; destruct (ty e') eqn:TE2; try discriminate; econstructor.
+        1,3,6: now apply IHgeneric_exp_sem1.
+        1,2,4: now apply IHgeneric_exp_sem2.
+        1,2: assumption.
+Qed.
